Add η-expansion to cumul
I have left some TODOs for later.

pcuic/theories/PCUICCumulativity.v
@@ -4,7 +4,7 @@ From Coq Require Import Bool String List Program BinPos Compare_dec.
 From MetaCoq.Template Require Import config utils AstUtils.
 From MetaCoq.PCUIC Require Import PCUICAst PCUICAstUtils PCUICInduction
      PCUICLiftSubst PCUICUnivSubst PCUICEquality PCUICTyping PCUICWeakeningEnv
-     PCUICWeakening PCUICClosed PCUICReduction.
+     PCUICWeakening PCUICClosed PCUICReduction PCUICPosition.
 Require Import ssreflect ssrbool.
 Require Import String.
 From MetaCoq Require Import LibHypsNaming.
@@ -14,24 +14,31 @@ Require Import CRelationClasses.
 Require Import Equations.Type.Relation Equations.Type.Relation_Properties.
 Require Import Equations.Prop.DepElim.
 
+Set Default Goal Selector "!".
+
 Reserved Notation " Σ ;;; Γ |- t == u " (at level 50, Γ, t, u at next level).
 
+(* TODO UPDATE *)
 Lemma cumul_alt `{cf : checker_flags} Σ Γ t u :
   Σ ;;; Γ |- t <= u <~> { v & { v' & (red Σ Γ t v * red Σ Γ u v' * leq_term (global_ext_constraints Σ) v v')%type } }.
 Proof.
   split.
-  { induction 1. exists t, u. intuition auto; constructor.
-    destruct IHX as (v' & v'' & (redv & redv') & leqv).
-    exists v', v''. intuition auto. now eapply red_step.
-    destruct IHX as (v' & v'' & (redv & redv') & leqv).
-    exists v', v''. intuition auto. now eapply red_step. }
-  { intros [v [v' [[redv redv'] Hleq]]]. apply red_alt in redv. apply red_alt in redv'.
+  - induction 1.
+    + exists t, u. intuition auto.
+    + destruct IHX as (v' & v'' & (redv & redv') & leqv).
+      exists v', v''. intuition auto. now eapply red_step.
+    + destruct IHX as (v' & v'' & (redv & redv') & leqv).
+      exists v', v''. intuition auto. now eapply red_step.
+    + destruct IHX as (v' & v'' & (redv & redv') & leqv).
+(*
+  - intros [v [v' [[redv redv'] Hleq]]]. apply red_alt in redv. apply red_alt in redv'.
     apply clos_rt_rt1n in redv.
     apply clos_rt_rt1n in redv'.
     induction redv. induction redv'. constructor; auto.
     econstructor 3; eauto.
-    econstructor 2; eauto. }
-Qed.
+    econstructor 2; eauto.
+Qed. *)
+Admitted.
 
 Lemma cumul_refl' {cf : checker_flags} Σ Γ t : Σ ;;; Γ |- t <= t.
 Proof.
@@ -48,8 +55,9 @@ Lemma red_cumul `{cf : checker_flags} {Σ : global_env_ext} {Γ t u} :
   Σ ;;; Γ |- t <= u.
 Proof.
   intros. apply red_alt in X. apply clos_rt_rt1n in X.
-  induction X. apply cumul_refl'.
-  econstructor 2; eauto.
+  induction X.
+  - apply cumul_refl'.
+  - econstructor 2. all: eauto.
 Qed.
 
 Lemma red_cumul_inv `{cf : checker_flags} {Σ : global_env_ext} {Γ t u} :
@@ -57,15 +65,16 @@ Lemma red_cumul_inv `{cf : checker_flags} {Σ : global_env_ext} {Γ t u} :
   Σ ;;; Γ |- u <= t.
 Proof.
   intros. apply red_alt in X. apply clos_rt_rt1n in X.
-  induction X. apply cumul_refl'.
-  econstructor 3; eauto.
+  induction X.
+  - apply cumul_refl'.
+  - econstructor 3. all: eauto.
 Qed.
 
 Lemma red_cumul_cumul `{cf : checker_flags} {Σ : global_env_ext} {Γ t u v} :
   red Σ Γ t u -> Σ ;;; Γ |- u <= v -> Σ ;;; Γ |- t <= v.
 Proof.
   intros. apply red_alt in X. apply clos_rt_rt1n in X.
-  induction X. auto.
+  induction X. 1: auto.
   econstructor 2; eauto.
 Qed.
 
@@ -73,8 +82,10 @@ Lemma red_cumul_cumul_inv `{cf : checker_flags} {Σ : global_env_ext} {Γ t u v}
   red Σ Γ t v -> Σ ;;; Γ |- u <= v -> Σ ;;; Γ |- u <= t.
 Proof.
   intros. apply red_alt in X. apply clos_rt_rt1n in X.
-  induction X. auto.
-  econstructor 3. eapply IHX. eauto. eauto.
+  induction X. 1: auto.
+  econstructor 3.
+  - eapply IHX. eauto.
+  - eauto.
 Qed.
 
 Lemma red_conv {cf:checker_flags} (Σ : global_env_ext) Γ t u : red Σ Γ t u -> Σ ;;; Γ |- t = u.
@@ -106,7 +117,9 @@ Lemma eq_term_mkApps `{checker_flags} φ f l f' l' :
 Proof.
   induction l in l', f, f' |- *; intro e; inversion_clear 1.
   - assumption.
-  - cbn. eapply IHl. constructor; assumption. assumption.
+  - cbn. eapply IHl.
+    + constructor; assumption.
+    + assumption.
 Qed.
 
 Lemma leq_term_App `{checker_flags} φ f f' :
@@ -123,13 +136,17 @@ Lemma leq_term_mkApps `{checker_flags} φ f l f' l' :
 Proof.
   induction l in l', f, f' |- *; intro e; inversion_clear 1.
   - assumption.
-  - cbn. apply IHl. constructor; try assumption. assumption.
+  - cbn. apply IHl.
+    + constructor; try assumption.
+    + assumption.
 Qed.
 
 Inductive conv_alt `{checker_flags} (Σ : global_env_ext) (Γ : context) : term -> term -> Type :=
 | conv_alt_refl t u : eq_term (global_ext_constraints Σ) t u -> Σ ;;; Γ |- t == u
 | conv_alt_red_l t u v : red1 Σ Γ t v -> Σ ;;; Γ |- v == u -> Σ ;;; Γ |- t == u
 | conv_alt_red_r t u v : Σ ;;; Γ |- t == v -> red1 (fst Σ) Γ u v -> Σ ;;; Γ |- t == u
+| conv_alt_eta_l t u v : eta_expands t v -> Σ ;;; Γ |- v == u -> Σ ;;; Γ |- t == u
+| conv_alt_eta_r t u v : Σ ;;; Γ |- t == v -> eta_expands u v -> Σ ;;; Γ |- t == u
 where " Σ ;;; Γ |- t == u " := (@conv_alt _ Σ Γ t u) : type_scope.
 
 Lemma red_conv_alt `{cf : checker_flags} Σ Γ t u :
@@ -137,9 +154,10 @@ Lemma red_conv_alt `{cf : checker_flags} Σ Γ t u :
   Σ ;;; Γ |- t == u.
 Proof.
   intros. apply red_alt in X. apply clos_rt_rt1n_iff in X.
-  induction X. constructor. apply eq_term_refl.
-  apply clos_rt_rt1n_iff in X. apply red_alt in X.
-  econstructor 2; eauto.
+  induction X.
+  - constructor. apply eq_term_refl.
+  - apply clos_rt_rt1n_iff in X. apply red_alt in X.
+    econstructor 2; eauto.
 Qed.
 Hint Resolve red_conv_alt.
 
@@ -163,19 +181,28 @@ Qed.
 
 Lemma conv_alt_sym `{cf : checker_flags} (Σ : global_env_ext) Γ t u :
   wf Σ ->
-  Σ ;;; Γ |- t == u -> Σ ;;; Γ |- u == t.
+  Σ ;;; Γ |- t == u ->
+  Σ ;;; Γ |- u == t.
 Proof.
   intros wfΣ X.
   induction X.
   - eapply eq_term_sym in e; now constructor.
-  - eapply red_conv_conv_inv. eapply red1_red in r. eauto. eauto.
-  - eapply red_conv_conv. eapply red1_red in r. eauto. eauto.
+  - eapply red_conv_conv_inv.
+    + eapply red1_red in r. eauto.
+    + eauto.
+  - eapply red_conv_conv.
+    + eapply red1_red in r. eauto.
+    + eauto.
+  - eapply conv_alt_eta_r. all: eassumption.
+  - eapply conv_alt_eta_l. all: eassumption.
 Qed.
 
+(* TODO UPDATE *)
 Lemma conv_alt_red {cf : checker_flags} {Σ : global_env_ext} {Γ : context} {t u : term} :
   Σ;;; Γ |- t == u <~> (∑ v v' : term, (red Σ Γ t v × red Σ Γ u v') × eq_term (global_ext_constraints Σ) v v').
 Proof.
-  split. induction 1. exists t, u; intuition auto.
+  split.
+  (* induction 1. exists t, u; intuition auto.
   destruct IHX as [? [? [? ?]]].
   exists x, x0; intuition auto. eapply red_step; eauto.
   destruct IHX as [? [? [? ?]]].
@@ -184,7 +211,8 @@ Proof.
   destruct X as [? [? [[? ?] ?]]].
   eapply red_conv_conv; eauto.
   eapply red_conv_conv_inv; eauto. now constructor.
-Qed.
+Qed. *)
+Admitted.
 
 Lemma conv_alt_cumul `{cf : checker_flags} (Σ : global_env_ext) Γ t u : wf Σ ->
   Σ ;;; Γ |- t == u -> Σ ;;; Γ |- t <= u.
@@ -198,8 +226,9 @@ Qed.
 Lemma conv_alt_conv `{cf : checker_flags} (Σ : global_env_ext) Γ t u : wf Σ ->
   Σ ;;; Γ |- t == u -> Σ ;;; Γ |- t = u.
 Proof.
-  intros wfΣ H. split. now apply conv_alt_cumul.
-  apply conv_alt_sym in H; auto. now apply conv_alt_cumul.
+  intros wfΣ H. split.
+  - now apply conv_alt_cumul.
+  - apply conv_alt_sym in H; auto. now apply conv_alt_cumul.
 Qed.
 
 (* TODO Probably not the right place
@@ -217,6 +246,10 @@ Proof.
     econstructor 2 ; eauto.
   - eapply PCUICWeakening.weakening_red1 in r ; auto.
     econstructor 3 ; eauto.
+  - eapply conv_alt_eta_l. 2: eassumption.
+    eapply weakening_eta_expands. assumption.
+  - eapply conv_alt_eta_r. 1: eassumption.
+    eapply weakening_eta_expands. assumption.
 Qed.
 
 Inductive conv_pb :=
@@ -246,7 +279,8 @@ Lemma conv_conv_r `{cf : checker_flags} :
 Proof.
   intros Σ [] Γ u v wfΣ h.
   - cbn. constructor. apply conv_alt_sym; auto.
-  - cbn. constructor. apply conv_alt_cumul. auto. now apply conv_alt_sym.
+  - cbn. constructor. apply conv_alt_cumul. 1: auto.
+    now apply conv_alt_sym.
 Qed.
 
 Lemma cumul_App_l `{cf : checker_flags} :
@@ -263,4 +297,12 @@ Proof.
     econstructor. assumption.
   - eapply cumul_red_r ; try eassumption.
     econstructor. assumption.
+  - eapply cumul_eta_l. 2: eassumption.
+    destruct e as [na [A [f [π [? ?]]]]]. subst.
+    exists na, A, f, (stack_cat π (App x ε)).
+    rewrite 2!zipc_stack_cat. cbn. intuition reflexivity.
+  - eapply cumul_eta_r. 1: eassumption.
+    destruct e as [na [A [f [π [? ?]]]]]. subst.
+    exists na, A, f, (stack_cat π (App x ε)).
+    rewrite 2!zipc_stack_cat. cbn. intuition reflexivity.
 Qed.
