pcuic/theories/PCUICTyping.v
@@ -512,6 +512,8 @@ Inductive cumul `{checker_flags} (Σ : global_env_ext) (Γ : context) : term -> 
 | cumul_refl t u : leq_term (global_ext_constraints Σ) t u -> Σ ;;; Γ |- t <= u
 | cumul_red_l t u v : red1 Σ.1 Γ t v -> Σ ;;; Γ |- v <= u -> Σ ;;; Γ |- t <= u
 | cumul_red_r t u v : Σ ;;; Γ |- t <= v -> red1 Σ.1 Γ u v -> Σ ;;; Γ |- t <= u
+| cumul_eta_l t u v : eta_expands t v -> Σ ;;; Γ |- v <= u -> Σ ;;; Γ |- t <= u
+| cumul_eta_r t u v : Σ ;;; Γ |- t <= v -> eta_expands u v -> Σ ;;; Γ |- t <= u
 
 where " Σ ;;; Γ |- t <= u " := (cumul Σ Γ t u) : type_scope.
 
